Use more implicit parameters

Wavelet/Compile.lean
@@ -9,9 +9,47 @@ namespace Wavelet.Compile
 
 open Op Seq Dataflow
 
-universe u
-variable (Op : Type u) (χ : Type u) (V S)
-variable [Arity Op] [DecidableEq χ] [instInterp : Interp Op V S]
+/--
+TODO: These are originally specified in the `where`
+clause of `compileExpr`, but I hit this issue:
+https://github.com/leanprover/lean4/issues/10559
+-/
+def compileExpr.allVarsExcept
+  [DecidableEq χ]
+  (definedVars vs : List χ)
+  (pathConds : List (Bool × ChanName χ)) :
+  Vector (ChanName χ) (definedVars.removeAll vs).length :=
+  (definedVars.removeAll vs).toVector.map (.var · pathConds)
+
+/-- Output channels of a compiled expression,
+essentially `return values ⊕ tail call arguments`. -/
+def compileExpr.exprOutputs
+  m n (pathConds : List (Bool × ChanName χ))
+  : Vector (ChanName χ) (n + (m + 1))
+  := (Vector.range n).map (ChanName.dest · pathConds) ++
+    (((Vector.range m).map (ChanName.tail_arg · pathConds)).push
+    (ChanName.tail_cond pathConds))
+
+def compileExpr.tailExprOutputs
+  m n (pathConds : List (Bool × ChanName χ))
+  : Vector (ChanName χ) (m + (n + 1))
+  := (Vector.range m).map (ChanName.tail_arg · pathConds) ++
+    ((Vector.range n).map (ChanName.dest · pathConds)).push
+    (ChanName.tail_cond pathConds)
+
+/-- Merge operator generated for each branching expression. -/
+def compileExpr.branchMerge
+  [Arity Op]
+  (m n : Nat)
+  (condName : ChanName χ)
+  (pathConds : List (Bool × ChanName χ))
+  : AtomicProc Op (ChanName χ) V :=
+  let leftConds := (true, condName) :: pathConds
+  let rightConds := (false, condName) :: pathConds
+  .merge (.merge_cond condName)
+    (compileExpr.exprOutputs m n leftConds)
+    (compileExpr.exprOutputs m n rightConds)
+    (compileExpr.exprOutputs m n pathConds)
 
 /--
 Compiles an expression to a list of atomic processes, with
@@ -22,79 +60,63 @@ chooses to perform a tail call (with `m` arguments) or return
 `n` final values.
 -/
 def compileExpr
+  [Arity Op] [InterpConsts V] [DecidableEq χ]
   (hnz : m > 0 ∧ n > 0)
   (definedVars : List χ)
   (pathConds : List (Bool × ChanName χ))
   : Expr Op χ m n → AtomicProcs Op (ChanName χ) V
   | .ret vars =>
-    let chans := varNames vars
-    let junks : Vector V m := Vector.replicate m (Interp.junkVal Op S)
-    let falseVal : V := Interp.fromBool Op S false
+    let chans := vars.map (.var · pathConds)
+    let junks : Vector V m := Vector.replicate m InterpConsts.junkVal
+    let falseVal : V := InterpConsts.fromBool false
     let consts : Vector V (m + 1) := junks ++ #v[falseVal]
     [
       .forwardc
         chans consts
-        (exprOutputs m n pathConds),
+        (compileExpr.exprOutputs m n pathConds),
       -- Discard all other variables
-      .sink (allVarsExcept vars.toList pathConds),
+      .sink (compileExpr.allVarsExcept definedVars vars.toList pathConds),
     ]
   | .tail vars =>
-    let chans := varNames vars
-    let junks : Vector V n := Vector.replicate n (Interp.junkVal Op S)
-    let trueVal : V := Interp.fromBool Op S true
+    let chans := vars.map (.var · pathConds)
+    let junks : Vector V n := Vector.replicate n InterpConsts.junkVal
+    let trueVal : V := InterpConsts.fromBool true
     let consts : Vector V (n + 1) := junks ++ #v[trueVal]
     [
       .forwardc
         chans consts
-        (exprOutputs' m n pathConds),
+        (compileExpr.tailExprOutputs m n pathConds),
       -- Discard all other variables
-      .sink (allVarsExcept vars.toList pathConds),
+      .sink (compileExpr.allVarsExcept definedVars vars.toList pathConds),
     ]
   | .op o args rets cont =>
-    let inputChans := varNames args
-    (.op o inputChans (varNames rets)) ::
-      compileExpr hnz (definedVars.removeAll args.toList ++ rets.toList) pathConds cont
+    let inputChans := args.map (.var · pathConds)
+    (.op o inputChans (rets.map (.var · pathConds))) ::
+      compileExpr hnz
+        (definedVars.removeAll args.toList ++ rets.toList)
+        pathConds cont
   | .br cond left right =>
-    let condChan := varName cond
+    let condChan := .var cond pathConds
     let leftConds := (true, condChan) :: pathConds
     let rightConds := (false, condChan) :: pathConds
-    let leftComp := compileExpr hnz (definedVars.removeAll [cond]) leftConds left
-    let rightComp := compileExpr hnz (definedVars.removeAll [cond]) rightConds right
+    let leftComp := compileExpr hnz
+      (definedVars.removeAll [cond]) leftConds left
+    let rightComp := compileExpr hnz
+      (definedVars.removeAll [cond]) rightConds right
     [
       -- Copy condition variables
       .fork condChan #v[.switch_cond condChan, .merge_cond condChan],
       -- Steer all live variables
       .switch (.switch_cond condChan)
-        (allVarsExcept [cond] pathConds)
-        (allVarsExcept [cond] leftConds)
-        (allVarsExcept [cond] rightConds),
+        (compileExpr.allVarsExcept definedVars [cond] pathConds)
+        (compileExpr.allVarsExcept definedVars [cond] leftConds)
+        (compileExpr.allVarsExcept definedVars [cond] rightConds),
     ] ++ leftComp ++ rightComp ++ [
       -- Merge tail call conditions, return values and tail call arguments
       -- from both branches. This is done at the end so that we can keep
       -- the graph as "acyclic" as possible.
-      brMerge m n condChan pathConds
+      compileExpr.branchMerge m n condChan pathConds
     ]
-  where
-    -- Current variable names
-    varName v := .var v pathConds
-    varNames {n} (vars : Vector χ n) := vars.map varName
-    allVarsExcept vs pathConds := (definedVars.removeAll vs).toVector.map (.var · pathConds)
-    exprOutputs m n pathConds :=
-      (Vector.range n).map (ChanName.dest · pathConds) ++
-      (((Vector.range m).map (ChanName.tail_arg · pathConds)).push
-       (ChanName.tail_cond pathConds))
-    -- Similar to `exprOutputs` but with `tail_arg`s and `dest`s swapped.
-    exprOutputs' m n pathConds :=
-      (Vector.range m).map (ChanName.tail_arg · pathConds) ++
-      ((Vector.range n).map (ChanName.dest · pathConds)).push
-        (ChanName.tail_cond pathConds)
-    brMerge m n condName pathConds :=
-      let leftConds := (true, condName) :: pathConds
-      let rightConds := (false, condName) :: pathConds
-      .merge (.merge_cond condName)
-        (exprOutputs m n leftConds)
-        (exprOutputs m n rightConds)
-        (exprOutputs m n pathConds)
 
 /--
 Compiles a function to a process with `m` inputs and `n` outputs.
@@ -103,10 +125,10 @@ Most of the compiled process should be a DAG, except for the back
 edges of channels with the name `.tail_cond []` or `.tail_arg i []`.
 -/
 def compileFn
+  [Arity Op] [DecidableEq χ] [InterpConsts V]
   (hnz : m > 0 ∧ n > 0)
   (fn : Fn Op χ m n) : Proc Op (ChanName χ) V m n
-  :=
-  {
+  := {
     inputs,
     outputs := (Vector.range n).map .final_tail_arg,
     atoms := initCarry false :: (bodyComp ++ resultSteers m n)
@@ -120,7 +142,8 @@ def compileFn
         inputs
         ((Vector.range m).map .final_tail_arg)
         (fn.params.map λ v => .var v [])
-    bodyComp := compileExpr Op χ V S hnz fn.params.toList [] fn.body
+    bodyComp := compileExpr hnz
+      fn.params.toList [] fn.body
     resultSteers m n := [
       .fork (.tail_cond []) #v[
         .tail_cond_carry,
