Wavelet/Dataflow.lean
@@ -7,13 +7,8 @@ namespace Wavelet.Dataflow
 
 open Op
 
-universe u
-variable (Op : Type u) (χ : Type u)
-variable [instArity : Arity Op]
-variable [DecidableEq χ]
-
 /-- Dataflow operators. -/
-inductive AtomicProc (V : Type u) where
+inductive AtomicProc (Op χ V : Type*) [Arity Op] where
   | op (op : Op) (inputs : Vector χ (Arity.ι op)) (outputs : Vector χ (Arity.ω op))
   | switch (decider : χ) (inputs : Vector χ n) (outputs₁ : Vector χ n) (outputs₂ : Vector χ n)
   | steer (flavor : Bool) (decider : χ) (inputs : Vector χ n) (outputs : Vector χ n)
@@ -34,30 +29,29 @@ inductive AtomicProc (V : Type u) where
     (inputs : Vector χ n) (consts : Vector V m) (outputs : Vector χ (n + m))
   | sink (inputs : Vector χ n)
 
-abbrev AtomicProcs V := List (AtomicProc Op χ V)
+abbrev AtomicProcs Op χ V [Arity Op] := List (AtomicProc Op χ V)
 
 /-- `Proc _ m n` is a process with `m` inputs and `n` outputs. -/
-structure Proc V (m : Nat) (n : Nat) where
+structure Proc Op χ V [Arity Op] (m : Nat) (n : Nat) where
   inputs : Vector χ m
   outputs : Vector χ n
   atoms : AtomicProcs Op χ V
 
-/- From this point onwards, assume a fixed operator semantics. -/
-variable (V S) [instInterp : Interp Op V S]
-
-abbrev ChanMap := χ → List V
+abbrev ChanMap χ V := χ → List V
 
 def ChanMap.empty : ChanMap χ V := λ _ => []
 
-def ChanMap.pushVal (name : χ) (val : V) (map : ChanMap χ V) : ChanMap χ V :=
+def ChanMap.pushVal [DecidableEq χ] (name : χ) (val : V) (map : ChanMap χ V) : ChanMap χ V :=
   λ n => if n = name then map n ++ [val] else map n
 
-def ChanMap.pushVals
+def ChanMap.pushVals [DecidableEq χ]
   (names : Vector χ n) (vals : Vector V n)
   (map : ChanMap χ V) : ChanMap χ V :=
-  (names.zip vals).foldl (λ map (n, v) => map.pushVal _ _ n v) map
+  (names.zip vals).foldl (λ map (n, v) => map.pushVal n v) map
 
 def ChanMap.popVal
+  {χ : Type*}
+  [DecidableEq χ]
   (name : χ)
   (map : ChanMap χ V) : Option (V × ChanMap χ V) :=
   match map name with
@@ -65,12 +59,13 @@ def ChanMap.popVal
   | v :: vs => some (v, λ n => if n = name then vs else map n)
 
 def ChanMap.popVals
+  [DecidableEq χ]
   (names : Vector χ n)
   (map : ChanMap χ V) : Option (Vector V n × ChanMap χ V)
   := (names.mapM popValM).run map
   where
     @[simp]
-    popValM : χ → StateT (ChanMap χ V) Option V := popVal χ V
+    popValM : χ → StateT (ChanMap χ V) Option V := popVal
 
 def ChanMap.IsSingleton (name : χ) (val : V) (map : ChanMap χ V) : Prop := map name = [val]
 
@@ -78,83 +73,89 @@ def ChanMap.IsEmpty (name : χ) (map : ChanMap χ V) : Prop := map name = []
 
 def ChanMap.getBuf (name : χ) (map : ChanMap χ V) : List V := map name
 
-structure Config m n where
+structure Config Op [Arity Op] χ V S m n where
   proc : Proc Op χ V m n
   chans : ChanMap χ V
   state : S
 
 /-- Initial process configuration. -/
 def Config.init
+  [Arity Op] [DecidableEq χ]
   (proc : Proc Op χ V m n)
   (state : S)
   (args : Vector V m) : Config Op χ V S m n
   := {
     proc,
-    chans := (ChanMap.empty _ _).pushVals _ _ proc.inputs args,
+    chans := ChanMap.empty.pushVals proc.inputs args,
     state,
   }
 
-inductive Config.Step : Config Op χ V S m n → Config Op χ V S m n → Prop where
+inductive Config.Step
+  {χ : Type u}
+  [Arity Op] [DecidableEq χ]
+  [InterpConsts V]
+  [InterpOp Op V S]
+  : Config Op χ V S m n → Config Op χ V S m n → Prop where
   | step_op {inputs : Vector χ (Arity.ι o)} :
     .op o inputs outputs ∈ c.proc.atoms →
-    c.chans.popVals _ _ inputs = some (inputVals, chans') →
-    (instInterp.interp o inputVals).run c.state = some (outputVals, state') →
+    c.chans.popVals inputs = some (inputVals, chans') →
+    (InterpOp.interp o inputVals).run c.state = some (outputVals, state') →
     Step c { c with
-      chans := chans'.pushVals _ _ outputs outputVals,
+      chans := chans'.pushVals outputs outputVals,
       state := state',
     }
   | step_switch
     {outputs₁ outputs₂ : Vector χ n} :
     .switch decider inputs outputs₁ outputs₂ ∈ c.proc.atoms →
-    c.chans.popVal _ _ decider = some (deciderVal, chans') →
-    chans'.popVals _ _ inputs = some (inputVals, chans'') →
-    instInterp.toBool deciderVal = some deciderBool →
+    c.chans.popVal decider = some (deciderVal, chans') →
+    chans'.popVals inputs = some (inputVals, chans'') →
+    InterpConsts.toBool deciderVal = some deciderBool →
     Step c { c with
       chans :=
         let outputs := if deciderBool then outputs₁ else outputs₂
-        chans''.pushVals _ _ outputs inputVals
+        chans''.pushVals outputs inputVals
     }
   | step_steer :
     .steer flavor decider inputs outputs ∈ c.proc.atoms →
-    c.chans.popVal _ _ decider = some (deciderVal, chans') →
-    chans'.popVals _ _ inputs = some (inputVals, chans'') →
-    instInterp.toBool deciderVal = some deciderBool →
+    c.chans.popVal decider = some (deciderVal, chans') →
+    chans'.popVals inputs = some (inputVals, chans'') →
+    InterpConsts.toBool deciderVal = some deciderBool →
     Step c { c with
       chans :=
         if deciderBool = flavor then
-          chans''.pushVals _ _ outputs inputVals
+          chans''.pushVals outputs inputVals
         else
           chans'',
     }
   | step_merge :
     .merge decider inputs₁ inputs₂ outputs ∈ c.proc.atoms →
-    c.chans.popVal _ _ decider = some (deciderVal, chans') →
-    instInterp.toBool deciderVal = some deciderBool →
-    chans'.popVals _ _
+    c.chans.popVal decider = some (deciderVal, chans') →
+    InterpConsts.toBool deciderVal = some deciderBool →
+    chans'.popVals
       (if deciderBool then inputs₁ else inputs₂)
       = some (inputVals, chans'') →
-    Step c { c with chans := chans''.pushVals _ _ outputs inputVals }
+    Step c { c with chans := chans''.pushVals outputs inputVals }
   | step_carry_init :
     c.proc.atoms = ctxLeft ++ [.carry false decider inputs₁ inputs₂ outputs] ++ ctxRight →
-    c.chans.popVals _ _ inputs₁ = some (inputVals, chans') →
+    c.chans.popVals inputs₁ = some (inputVals, chans') →
     Step c { c with
       proc := { c.proc with
         atoms := ctxLeft ++ [.carry true decider inputs₁ inputs₂ outputs] ++ ctxRight,
       },
-      chans := chans'.pushVals _ _ outputs inputVals,
+      chans := chans'.pushVals outputs inputVals,
     }
   | step_carry_true :
     c.proc.atoms = ctxLeft ++ [.carry true decider inputs₁ inputs₂ outputs] ++ ctxRight →
-    c.chans.popVal _ _ decider = some (deciderVal, chans') →
-    instInterp.toBool deciderVal = some true →
-    chans'.popVals _ _ inputs₂ = some (inputVals, chans'') →
+    c.chans.popVal decider = some (deciderVal, chans') →
+    InterpConsts.toBool deciderVal = some true →
+    chans'.popVals inputs₂ = some (inputVals, chans'') →
     Step c { c with
-      chans := chans''.pushVals _ _ outputs inputVals,
+      chans := chans''.pushVals outputs inputVals,
     }
   | step_carry_false :
     c.proc.atoms = ctxLeft ++ [.carry true decider inputs₁ inputs₂ outputs] ++ ctxRight →
-    c.chans.popVal _ _ decider = some (deciderVal, chans') →
-    instInterp.toBool deciderVal = some false →
+    c.chans.popVal decider = some (deciderVal, chans') →
+    InterpConsts.toBool deciderVal = some false →
     Step c { c with
       proc := { c.proc with
         atoms := ctxLeft ++ [.carry false decider inputs₁ inputs₂ outputs] ++ ctxRight,
@@ -163,50 +164,41 @@ inductive Config.Step : Config Op χ V S m n → Config Op χ V S m n → Prop w
     }
   | step_forward :
     .forward inputs outputs ∈ c.proc.atoms →
-    c.chans.popVals _ _ inputs = some (inputVals, chans') →
+    c.chans.popVals inputs = some (inputVals, chans') →
     Step c { c with
-      chans := chans'.pushVals _ _ outputs inputVals,
+      chans := chans'.pushVals outputs inputVals,
     }
   | step_fork :
     .fork input outputs ∈ c.proc.atoms →
-    c.chans.popVal _ _ input = some (inputVal, chans') →
+    c.chans.popVal input = some (inputVal, chans') →
     Step c { c with
-      chans := chans'.pushVals _ _ outputs (Vector.replicate _ inputVal),
+      chans := chans'.pushVals outputs (Vector.replicate _ inputVal),
     }
   | step_const :
     .const val act outputs ∈ c.proc.atoms →
-    c.chans.popVal _ _ act = some (actVal, chans') →
+    c.chans.popVal act = some (actVal, chans') →
     Step c { c with
-      chans := chans'.pushVals _ _ outputs (Vector.replicate _ val),
+      chans := chans'.pushVals outputs (Vector.replicate _ val),
     }
   | step_forwardc :
     .forwardc inputs consts outputs ∈ c.proc.atoms →
-    c.chans.popVals _ _ inputs = some (inputVals, chans') →
+    c.chans.popVals inputs = some (inputVals, chans') →
     Step c { c with
-      chans := chans'.pushVals _ _ outputs (inputVals ++ consts),
+      chans := chans'.pushVals outputs (inputVals ++ consts),
     }
   | step_sink :
     .sink inputs ∈ c.proc.atoms →
-    c.chans.popVals _ _ inputs = some (inputVals, chans') →
+    c.chans.popVals inputs = some (inputVals, chans') →
     Step c { c with chans := chans' }
 
-def Config.StepPlus {m n} := @Relation.TransGen (Config Op χ V S m n) (Step Op χ V S)
-def Config.StepStar {m n} := @Relation.ReflTransGen (Config Op χ V S m n) (Step Op χ V S)
+def Config.StepPlus
+  {Op χ V S m n}
+  [Arity Op] [InterpConsts V] [InterpOp Op V S] [DecidableEq χ] :=
+  @Relation.TransGen (Config Op χ V S m n) Step
 
-/- Some alternative forms of stepping. -/
-
-theorem step_eq
-  (hstep : Config.Step Op χ V S c₁ c₂)
-  (heq : c₂ = c₂') :
-  Config.Step _ _ _ _ c₁ c₂' := by
-  simp [heq] at hstep
-  exact hstep
-
-theorem step_plus_eq
-  (hstep : Config.StepPlus Op χ V S c₁ c₂)
-  (heq : c₂ = c₂') :
-  Config.StepPlus _ _ _ _ c₁ c₂' := by
-  simp [heq] at hstep
-  exact hstep
+def Config.StepStar
+  {Op χ V S m n}
+  [Arity Op] [InterpConsts V] [InterpOp Op V S] [DecidableEq χ] :=
+  @Relation.ReflTransGen (Config Op χ V S m n) Step
 
 end Wavelet.Dataflow
