Wavelet/Op.lean
@@ -2,24 +2,26 @@
 
 namespace Wavelet.Op
 
-universe u
-variable (Op : Type u) (χ : Type u)
-
 /-- Assigns arities to each operator. -/
-class Arity where
+class Arity Op where
   ι : Op → Nat
   ω : Op → Nat
 
-variable [Arity Op]
-
-/-- Interpretation of an operator set as concrete values. -/
-class Interp (V S : Type u) where
-  interp : (op : Op) → Vector V (Arity.ι op) → StateT S Option (Vector V (Arity.ω op))
+/-- Some constants used in compilation. -/
+class InterpConsts (V : Type v) where
+  -- Placeholder value
+  junkVal : V
+  -- Booleans
   toBool : V → Option Bool
   fromBool : Bool → V
-  -- Some constants used in compilation
-  junkVal : V
   unique_fromBool_toBool : ∀ b, toBool (fromBool b) = some b
   unique_toBool_fromBool : ∀ b v, toBool v = some b → v = fromBool b
+
+/--
+Interpretation of operators.
+TODO: `V` and `S` are in the same universe due to the type of `StateT`.
+-/
+class InterpOp Op (V S : Type v) [Arity Op] where
+  interp : (op : Op) → Vector V (Arity.ι op) → StateT S Option (Vector V (Arity.ω op))
 
 end Wavelet.Op
