Wavelet/Simulation/Invariants.lean
@@ -12,21 +12,21 @@ namespace Wavelet.Simulation.Invariants
 open Op Seq Dataflow Compile
 
 def varsToChans
-  [Arity Op] [instInterp : Interp Op V S]
+  [Arity Op] [DecidableEq χ] [InterpConsts V]
   (ec : Seq.Config Op χ V S m n) : ChanMap (ChanName χ) V :=
   λ name =>
     match name with
     | .var v pathConds =>
       if pathConds = ec.pathConds then
-        if let some val := ec.vars.getVar _ _ v then
+        if let some val := ec.vars.getVar v then
           [val]
         else []
       else []
     | .merge_cond v =>
       if (true, v) ∈ ec.pathConds then
-        [instInterp.fromBool true]
+        [InterpConsts.fromBool true]
       else if (false, v) ∈ ec.pathConds then
-        [instInterp.fromBool false]
+        [InterpConsts.fromBool false]
       else []
     | .final_dest i =>
       -- Corresponding final return values
@@ -44,7 +44,7 @@ def HasMerges
   List (Bool × ChanName χ) → Prop
   | [] => True
   | (_, chan) :: rest =>
-    (compileExpr.brMerge _ _ _ m n chan rest ∈ atoms) ∧
+    (compileExpr.branchMerge m n chan rest ∈ atoms) ∧
     HasMerges m n atoms rest
 
 @[grind]
@@ -56,15 +56,15 @@ def OrderedPathConds (pathConds : List (Bool × ChanName χ)) : Prop :=
 to the compiled expressions/fns. -/
 @[grind]
 def HasCompiledProcs
-  [Arity Op] [Interp Op V S] [DecidableEq χ]
+  [Arity Op] [DecidableEq χ] [InterpConsts V]
   (hnz : m > 0 ∧ n > 0)
   (ec : Seq.Config Op χ V S m n)
   (pc : Dataflow.Config Op (ChanName χ) V S m n) : Prop :=
   ∃ (rest : AtomicProcs Op (ChanName χ) V)
     (carryInLoop : Bool)
     (ctxLeft ctxCurrent ctxRight : AtomicProcs Op (ChanName χ) V),
-    pc.proc.atoms = compileFn.initCarry _ _ _ ec.fn carryInLoop :: rest ∧
-    (compileFn Op χ V S hnz ec.fn).atoms = compileFn.initCarry _ _ _ ec.fn false :: rest ∧
+    pc.proc.atoms = compileFn.initCarry ec.fn carryInLoop :: rest ∧
+    (compileFn hnz ec.fn).atoms = compileFn.initCarry ec.fn false :: rest ∧
     rest = ctxLeft ++ ctxCurrent ++ ctxRight ∧
     (∀ vals, ec.expr = .ret vals → ¬ carryInLoop ∧
       ctxCurrent = [] ∧
@@ -72,12 +72,12 @@ def HasCompiledProcs
       ec.definedVars = [] ∧
       ec.pathConds = []) ∧
     (∀ expr, ec.expr = .cont expr → carryInLoop ∧
-      expr.WellFormed _ _ ec.definedVars ∧
-      compileExpr Op χ V S hnz ec.definedVars ec.pathConds expr = ctxCurrent)
+      expr.WellFormed ec.definedVars ∧
+      compileExpr hnz ec.definedVars ec.pathConds expr = ctxCurrent)
 
 @[grind]
 def SimRel
-  [Arity Op] [Interp Op V S] [DecidableEq χ]
+  [Arity Op] [DecidableEq χ] [InterpConsts V]
   (hnz : m > 0 ∧ n > 0)
   (ec : Seq.Config Op χ V S m n)
   (pc : Dataflow.Config Op (ChanName χ) V S m n) : Prop :=
@@ -85,7 +85,7 @@ def SimRel
   -- Some invariants about the correspondence between variables and channels
   pc.chans = varsToChans ec ∧
   ec.definedVars.Nodup ∧
-  (∀ var, var ∈ ec.definedVars ↔ ∃ val, ec.vars.getVar _ _ var = some val) ∧
+  (∀ var, var ∈ ec.definedVars ↔ ∃ val, ec.vars.getVar var = some val) ∧
   OrderedPathConds ec.pathConds ∧
   -- No path condition are pushed twice
   (ec.pathConds.map Prod.snd).Nodup ∧
@@ -97,8 +97,9 @@ def SimRel
 /-! Utility functions to extract facts from the simulation relation. -/
 section Utilities
 
-variable {Op χ V S}
-variable [Arity Op] [Interp Op V S] [DecidableEq χ]
+variable {Op χ : Type*}
+variable {V S : Type u}
+variable [Arity Op] [DecidableEq χ] [InterpConsts V]
 variable {ec : Seq.Config Op χ V S m n}
 variable {pc : Dataflow.Config Op (ChanName χ) V S m n}
 variable {hnz : m > 0 ∧ n > 0}
@@ -115,17 +116,17 @@ def SimRel.wf_fn : ec.fn.WellFormed := by
 def SimRel.defined_vars_nodup : ec.definedVars.Nodup := hsim.2.2.1
 
 def SimRel.defined_vars_to_get_var :
-  var ∈ ec.definedVars → ∃ val, ec.vars.getVar _ _ var = some val := by
+  var ∈ ec.definedVars → ∃ val, ec.vars.getVar var = some val := by
   have ⟨_, _, _, h, _⟩ := hsim
   apply (h var).mp
 
 def SimRel.get_var_to_defined_vars :
-  (∃ val, ec.vars.getVar _ _ var = some val) → var ∈ ec.definedVars := by
+  (∃ val, ec.vars.getVar var = some val) → var ∈ ec.definedVars := by
   have ⟨_, _, _, h, _⟩ := hsim
   apply (h var).mpr
 
 def SimRel.defined_vars_iff_get_var
-  : var ∈ ec.definedVars ↔ ∃ val, ec.vars.getVar _ _ var = some val := by
+  : var ∈ ec.definedVars ↔ ∃ val, ec.vars.getVar var = some val := by
   have ⟨_, _, _, h, _⟩ := hsim
   exact h var
 
